13MachineCode/MachineCode.thy
@@ -5,71 +5,41 @@ begin
 datatype reg = R1 | R2 | R3 | R4 | R5
 
 datatype mach = 
-  LDI reg nat   (* $R := k *)
-  | LOD reg reg (* $R\<^sub>1 := M[$R\<^sub>2] *)
-  | STO reg reg (* M[$R\<^sub>1] := $R\<^sub>2 *)
-  | STI reg nat (* M[$R] := k *)
-  | MOV reg reg (* $R\<^sub>1 := $R\<^sub>2 *)
-  | ADD reg nat (* $R := $R + k *)
-  | SUB reg nat (* $R := $R - k *)
-  | JMP reg     (* $PC := $R (indirect jump) *)
+  MOV reg reg    (* $R\<^sub>1 := $R\<^sub>2 *)
+  | LOD reg reg  (* $R\<^sub>1 := M[$R\<^sub>2] *)
+  | LODI reg nat (* $R := k *)
+  | STO reg reg  (* M[$R\<^sub>1] := $R\<^sub>2 *)
+  | STOI reg nat (* M[$R] := k *)
+  | ADD reg reg  (* $R\<^sub>1 := $R\<^sub>1 + $R\<^sub>2 *)
+  | ADDI reg nat (* $R := $R + k *)
+  | SUB reg reg  (* $R\<^sub>1 := $R\<^sub>1 - $R\<^sub>2 *)
+  | SUBI reg nat (* $R := $R - k *)
+  | JMP reg      (* $PC := $R (indirect jump) *)
+  | JMPI nat     (* $PC := k (direct jump) *)
 
 datatype mach_state = MS "reg \<Rightarrow> nat" "nat \<Rightarrow> nat" nat
 
-inductive evalm :: "mach list \<Rightarrow> mach_state \<Rightarrow> mach_state \<Rightarrow> bool" (infix "\<tturnstile> _ \<leadsto>\<^sub>m" 50) where 
-  evm_ldi [simp]: "cd ! pc = LDI r k \<Longrightarrow> 
-    cd \<tturnstile> MS rs mem (Suc pc) \<leadsto>\<^sub>m MS (rs(r := k)) mem pc"
-| evm_lod [simp]: "cd ! pc = LOD r ptr \<Longrightarrow> 
-    cd \<tturnstile> MS rs mem (Suc pc) \<leadsto>\<^sub>m MS (rs(r := mem (rs ptr))) mem pc"
-| evm_sto [simp]: "cd ! pc = STO ptr r \<Longrightarrow> 
-    cd \<tturnstile> MS rs mem (Suc pc) \<leadsto>\<^sub>m MS rs (mem(rs ptr := rs r)) pc"
-| evm_sti [simp]: "cd ! pc = STI ptr k \<Longrightarrow> 
-    cd \<tturnstile> MS rs mem (Suc pc) \<leadsto>\<^sub>m MS rs (mem(rs ptr := k)) pc"
-| evm_mov [simp]: "cd ! pc = MOV r1 r2 \<Longrightarrow> 
-    cd \<tturnstile> MS rs mem (Suc pc) \<leadsto>\<^sub>m MS (rs(r1 := rs r2)) mem pc"
-| evm_add [simp]: "cd ! pc = ADD r k \<Longrightarrow> 
-    cd \<tturnstile> MS rs mem (Suc pc) \<leadsto>\<^sub>m MS (rs(r := rs r + k)) mem pc"
-| evm_sub [simp]: "cd ! pc = SUB r k \<Longrightarrow> 
-    cd \<tturnstile> MS rs mem (Suc pc) \<leadsto>\<^sub>m MS (rs(r := rs r - k)) mem pc"
-| evm_jmp [simp]: "cd ! pc = JMP r \<Longrightarrow> 
-    cd \<tturnstile> MS rs mem (Suc pc) \<leadsto>\<^sub>m MS (rs(r := 0)) mem (rs r)"
+primrec evalm_step :: "mach \<Rightarrow> (reg \<Rightarrow> nat) \<Rightarrow> (nat \<Rightarrow> nat) \<Rightarrow> nat \<Rightarrow> mach_state" where
+  "evalm_step (MOV r r') rs mem pc = MS (rs(r := rs r')) mem pc"
+| "evalm_step (LOD r r') rs mem pc = MS (rs(r := mem (rs r'))) mem pc"
+| "evalm_step (LODI r k) rs mem pc = MS (rs(r := k)) mem pc"
+| "evalm_step (STO r r') rs mem pc = MS rs (mem(rs r := rs r')) pc"
+| "evalm_step (STOI r k) rs mem pc = MS rs (mem(rs r := k)) pc"
+| "evalm_step (ADD r r') rs mem pc = MS (rs(r := rs r + rs r')) mem pc"
+| "evalm_step (ADDI r k) rs mem pc = MS (rs(r := rs r + k)) mem pc"
+| "evalm_step (SUB r r') rs mem pc = MS (rs(r := rs r - rs r')) mem pc"
+| "evalm_step (SUBI r k) rs mem pc = MS (rs(r := rs r - k)) mem pc"
+| "evalm_step (JMP r)    rs mem pc = MS (rs(r := 0)) mem (rs r)"
+| "evalm_step (JMPI k)   rs mem pc = MS rs mem k"
+
+fun evalm :: "mach list \<Rightarrow> mach_state \<rightharpoonup> mach_state" where 
+  "evalm cd (MS rs mem 0) = None"
+| "evalm cd (MS rs mem (Suc pc)) = Some (evalm_step (cd ! pc) rs mem pc)"
+
+abbreviation evalm_relation :: "mach list \<Rightarrow> mach_state \<Rightarrow> mach_state \<Rightarrow> bool" (infix "\<tturnstile> _ \<leadsto>\<^sub>m" 50) where 
+  "cd \<tturnstile> \<Sigma> \<leadsto>\<^sub>m \<Sigma>' \<equiv> (evalm cd \<Sigma> = Some \<Sigma>')"
 
 theorem determinismm: "cd \<tturnstile> \<Sigma> \<leadsto>\<^sub>m \<Sigma>' \<Longrightarrow> cd \<tturnstile> \<Sigma> \<leadsto>\<^sub>m \<Sigma>'' \<Longrightarrow> \<Sigma>' = \<Sigma>''"
-proof (induction cd \<Sigma> \<Sigma>' rule: evalm.induct)
-  case (evm_ldi cd pc r k rs mem)
-  from evm_ldi(2, 1) show ?case 
-    by (induction cd "MS rs mem (Suc pc)" \<Sigma>'' rule: evalm.induct) simp_all
-next
-  case (evm_lod cd pc r ptr rs mem)
-  from evm_lod(2, 1) show ?case 
-    by (induction cd "MS rs mem (Suc pc)" \<Sigma>'' rule: evalm.induct) simp_all
-next
-  case (evm_sto cd pc ptr r rs mem)
-  from evm_sto(2, 1) show ?case 
-    by (induction cd "MS rs mem (Suc pc)" \<Sigma>'' rule: evalm.induct) simp_all
-next
-  case (evm_sti cd pc ptr k rs mem)
-  from evm_sti(2, 1) show ?case 
-    by (induction cd "MS rs mem (Suc pc)" \<Sigma>'' rule: evalm.induct) simp_all
-next
-  case (evm_mov cd pc r1 r2 rs mem)
-  from evm_mov(2, 1) show ?case 
-    by (induction cd "MS rs mem (Suc pc)" \<Sigma>'' rule: evalm.induct) simp_all
-next
-  case (evm_add cd pc r k rs mem)
-  from evm_add(2, 1) show ?case 
-    by (induction cd "MS rs mem (Suc pc)" \<Sigma>'' rule: evalm.induct) simp_all
-next
-  case (evm_sub cd pc r k rs mem)
-  from evm_sub(2, 1) show ?case 
-    by (induction cd "MS rs mem (Suc pc)" \<Sigma>'' rule: evalm.induct) simp_all
-next
-  case (evm_jmp cd pc r rs mem)
-  from evm_jmp(2, 1) show ?case 
-    by (induction cd "MS rs mem (Suc pc)" \<Sigma>'' rule: evalm.induct) simp_all
-qed
-
-lemma [simp]: "cd ! pc = MOV R5 R5 \<Longrightarrow> cd \<tturnstile> MS rs mem (Suc pc) \<leadsto>\<^sub>m MS rs mem pc"
-  using evm_mov by fastforce
+  by simp
 
 end
