Readme.md
@@ -20,4 +20,5 @@ Refactorings:
 - Make late stage closures (post bytecode) a single parametric datatype?
 - Clean up isabelle - declare x.simps[intros], assumes/shows, patterns in pfs
 - Use ints insted of nats for machine code
-- Flip environment layout
+- Alter environment layout to make lookups more efficient
+- Make consts use ints instead of nats?
